upgraded RG to allow edge labels

project/relational_graph_IG_basic_operations.v
@@ -16,7 +16,7 @@ Require Import Coq.Sets.Ensembles.
 Require Import MyProject.project.util.NatSet.
 
 
-(* Defines the basic IG functions in terms of an RG *)
+(* Defines the IG_basic functions in terms of an RG (without multigraph) soon to be outclassed by relational_graph_IG_operations*)
   (* {-# MINIMAL empty, isEmpty, match, mkGraph, labNodes #-} *)
 
 
@@ -30,26 +30,28 @@ Definition RG_isEmpty (rg : RG nat) : Prop :=
 
 
 
-(* Helper for matsh *)
+(* Helper for match *)
+(* Removes a node from the nodeset and any edges *)
 Definition _eliminate (node : Node) (rg : RG nat) : RG nat.
 Proof.
   refine {|
-      RG_nodes := Subtract nat (rg.(RG_nodes)) node;
-      RG_edges := fun (n0 n1 : nat) => n0 <> node /\ n1 <> node /\  rg.(RG_edges) n0 n1;
+      RG_nodes := Subtract nat rg.(RG_nodes) node;
+      RG_edges := fun (n1 n2 : nat) => n1 <> node /\ n2 <> node /\  rg.(RG_edges) n1 n2;
       RG_valid := _
   |}.
   RG_valid_prover_with rg.
-  - unfold not. intros. inversion H2. congruence.
-  - unfold not. intros. inversion H2. congruence.
+  - unfold not. intros. inversion H3. congruence.
+  - unfold not. intros. inversion H3. congruence.
 Defined.
 
+(* Checks if the node is in the RG (the Prop return) and returns two sets of alls incoming neighbors and outgoing neighbors *)
 Definition _getFromsAndTos (node : Node) (rg : RG nat) : Prop * (Ensemble nat * Ensemble nat) :=
   (rg.(RG_nodes) node, ((fun (from : nat) => rg.(RG_edges) from node), (fun (to : nat) => rg.(RG_edges) node to)))
 .
 
 
 (* (Ensemble nat * Ensemble nat) is not a relation, it is two _independent_ sets of from- and to- neighbors *)
-Definition RG_matsh (node : Node) (rg : RG nat) : (Prop * (Ensemble nat * Ensemble nat)) * RG nat :=
+Definition RG_match (node : Node) (rg : RG nat) : (Prop * (Ensemble nat * Ensemble nat)) * RG nat :=
   (_getFromsAndTos node rg, _eliminate node rg)
 .
 
@@ -73,10 +75,10 @@ Definition _insNodes (nodes : list Node) (rg : RG nat) : RG nat :=
 (* If one of the nodes of the edge does not exist, nothing happens *)
 Definition _insEdge (edge : (Node * Node)) (rg : RG nat) : RG nat.
 Proof.
-  destruct edge as [node0 node1].
+  destruct edge as [node1 node2].
     refine {|
       RG_nodes := rg.(RG_nodes);
-      RG_edges := fun (n0 n1 : nat) => (n0 = node0 /\ n1 = node1 /\ rg.(RG_nodes) node0 /\ rg.(RG_nodes) node1) \/  rg.(RG_edges) n0 n1;
+      RG_edges := fun (n1 n2 : nat) => (n1 = node1 /\ n2 = node2 /\ rg.(RG_nodes) node1 /\ rg.(RG_nodes) node2) \/  rg.(RG_edges) n1 n2;
       RG_valid := _
   |}.
   RG_valid_prover_with rg.
@@ -91,5 +93,6 @@ Definition _insEdges (edges : list (Node * Node)) (rg : RG nat) : RG nat :=
 Definition RG_mkGraph (nodes : list Node) (edges : list (Node * Node)) : RG nat :=
   _insEdges edges (_insNodes nodes RG_empty).
  
+
 Definition RG_labNodes (rg : RG nat) : Ensemble Node :=
   rg.(RG_nodes).
