project/relational_graph_IG_operations_theory.v
@@ -1,0 +1,117 @@
+Require Import String.
+Require Import Coq.Arith.Arith.
+Open Scope string_scope.
+
+Require Import List.
+Require Import Bool.
+Import ListNotations.
+
+Require Import MyProject.project.util.util.
+
+(* Require Import MyProject.project.relational_graph.
+Require Import MyProject.project.relational_graph_theory. *)
+Require Import MyProject.project.relational_graph_IG_operations.
+
+Require Import Coq.Sets.Ensembles.
+
+Require Import MyProject.project.util.NatSet.
+
+
+Open Scope nat_scope.
+
+(* Specifies behavior of IH functions on an (edge-label compatible) RG via equational specification *)
+
+
+(* Here start "meaningful statements" *)
+
+(* 5 statements on inserting (helpers for mkGraph): update, insEdge, insEdges, insNode, insNodes *)
+
+Lemma RG_insEdge_does_not_add_node : forall (A B : Type) (edge : (Edge A B)) (rg : RG A B),
+  RG_labNodes (_insEdge edge rg) = RG_labNodes rg.
+Proof.
+Admitted.
+  (* intros. simpl. unfold RG_labNodes. unfold _insEdge. destruct edge. simpl. reflexivity. *)
+
+
+Lemma RG_insEdges_does_not_add_nodes : forall (A B : Type) (edges : list (@Edge A B)) (rg : RG A B),
+  RG_labNodes (_insEdges edges rg) = RG_labNodes rg.
+Proof.
+Admitted.
+
+
+Lemma RG_insNode_any_ins_node : forall (A B : Type) (node : A) (rg : RG A B),
+  RG_labNodes (_insNode node rg) = _customEnsembleAdd node (RG_labNodes rg).
+Proof.
+Admitted.
+
+
+
+
+Lemma RG_insNodes_any_ins_all_nodes : forall (A B : Type) (nodes : list A) (rg : RG A B),
+  RG_labNodes (_insNodes nodes rg) = Union A (_listToEnsemble nodes) (RG_labNodes rg).
+Proof.
+Admitted.
+
+
+
+Lemma RG_insEdge_on_empty_is_empty : forall (A B : Type) (edge : (Edge A B)),
+  _insEdge edge RG_empty = RG_empty.
+Proof.
+Admitted.
+
+
+Lemma RG_insEdges_on_empty_is_empty : forall (A B : Type) (edges : list (Edge A B)),
+  _insEdges edges RG_empty = RG_empty.
+(* This proof is very similar to "insEdges_does_not_add_nodes", but using it here it is more complicated than just doing it again  *)
+Proof.
+Admitted.
+
+
+
+(* "big" statement: *)
+Theorem RG_mkGraph_any_ins_all_nodes : forall (A B : Type) (nodes : list A) (edges : list (Edge A B)),
+  RG_labNodes (RG_mkGraph nodes edges) = _listToEnsemble nodes.
+Proof.
+Admitted.
+
+
+Theorem RG_empty_isEmpty : forall (A B : Type), RG_isEmpty (@RG_empty A B).
+Proof.
+  compute. reflexivity.
+Qed.
+
+Theorem RG_labNodes_empty_nil : forall (A B : Type), RG_labNodes (@RG_empty A B) = Empty_set A.
+Proof.
+Admitted.
+
+
+
+Theorem RG_non_empty_isEmpty_false : forall (A B : Type) (nodes : list A) (edges : list (Edge A B)),
+  length nodes <> 0 <-> not (RG_isEmpty ((RG_mkGraph nodes edges))).
+Proof.
+Admitted.
+
+
+
+
+Theorem RG_match_empty_is_nothing : forall (A B : Type) (node : A),
+  RG_match node (@RG_empty A B) = ((False, (fun x y => False, node, fun x y => False)), RG_empty).
+Proof.
+Admitted.
+
+
+
+
+
+(* Theorem RG_spec4 : forall (A B : Type) (node : A) (nodes : list A) (edges : list (Edge A B)), 
+  List.In node nodes -> exists froms tos, RG_match node (RG_mkGraph nodes edges) =
+  ((True, (froms, tos)), RG_mkGraph (filter (fun n => negb (node =? n)) nodes) (filter (fun '(from, to) => negb ((from =? node) || (to =? node))) edges)).
+(* This is not even a complete specification and it looks like a hard one to prove... *)
+Proof.
+Admitted. *)
+
+
+Theorem RG_spec5 : forall (A B : Type) (node : A) (nodes : list A) (edges : list (Edge A B)), 
+  not (List.In node nodes) -> RG_match node (RG_mkGraph nodes edges) = ((False, (fun x y => False, node, fun x y => False)), RG_mkGraph nodes edges).
+Proof.
+Admitted.
